@prefix : <http://leduc.gamsau.archi.fr/>.
@prefix dct: <http://purl.org/dc/terms/>.
@prefix foaf: <http://xmlns.com/foaf/spec/>.
@prefix iqvoc: <http://try.iqvoc.net/schema#>.
@prefix owl: <http://www.w3.org/2002/07/owl#>.
@prefix rdf: <http://www.w3.org/1999/02/22-rdf-syntax-ns#>.
@prefix rdfs: <http://www.w3.org/2000/01/rdf-schema#>.
@prefix schema: <http://leduc.gamsau.archi.fr/schema#>.
@prefix skos: <http://www.w3.org/2004/02/skos/core#>.
@prefix void: <http://rdfs.org/ns/void#>.

:_72b9ad8d a skos:Concept;
           skos:topConceptOf :scheme;
           skos:inScheme :scheme;
           skos:prefLabel "Crack & Deformation"@en;
           skos:prefLabel "Fissure & Déformation"@fr;
           skos:narrower :_7eb0c1ad;
           skos:narrower :_bb1ba8aa;
           skos:changeNote [
    dct:creator "Admin Istrator";
    dct:modified "2017-05-24T10:06:07+00:00"
];
           skos:changeNote [
    dct:creator "Nicola Carboni";
    dct:modified "2017-05-24T15:59:54+00:00"
].
:_7eb0c1ad a skos:Concept;
           skos:inScheme :scheme;
           skos:prefLabel "Crack"@en;
           skos:prefLabel "Fissure"@fr;
           skos:altLabel "Fissure"@en;
           skos:altLabel "Fault"@en;
           skos:altLabel "Joint"@en;
           skos:altLabel "Raquelure"@fr;
           skos:altLabel "fêlure"@fr;
           skos:altLabel "Fente"@fr;
           skos:altLabel "Fendage"@fr;
           skos:altLabel "Faille"@fr;
           skos:altLabel "Diaclase"@fr;
           skos:broader :_72b9ad8d;
           skos:narrower :_ea3a5e3f;
           skos:narrower :_ca0dece9;
           skos:narrower :_7285fd07;
           skos:narrower :_94ebf59e;
           skos:narrower :_bfe46976;
           skos:broader :_72b9ad8d;
           skos:changeNote [
    dct:creator "Nicola Carboni";
    dct:modified "2017-05-24T16:00:20+00:00"
];
           skos:definition "Individual fissure, clearly visible by the naked eye, resulting from separation of one part from another."@en;
           skos:definition "Une fissure est un plan de rupture vu en coupe qui résulte de la séparation d’une pierre en deux par- ties."@fr.
:_ea3a5e3f a skos:Concept;
           skos:inScheme :scheme;
           skos:prefLabel "Fracture"@en;
           skos:prefLabel "Fracture"@fr;
           skos:broader :_7eb0c1ad;
           skos:definition "Crack that crosses completely the stone piece"@en;
           skos:definition "Fissure traversant complètement une pierre."@fr.
:_ca0dece9 a skos:Concept;
           skos:inScheme :scheme;
           skos:prefLabel "Craquele"@en;
           skos:prefLabel "Craquellement"@fr;
           skos:altLabel "crack network"@en;
           skos:broader :_7eb0c1ad;
           skos:changeNote [
    dct:creator "Nicola Carboni";
    dct:modified "2017-05-24T16:09:41+00:00"
];
           skos:definition "Network of minor cracks also called crack network . The term crazing is not appropriate for stone, as this term should be used for describing the development of a crack network on glazed terracotta."@en;
           skos:definition "Réseau de fissures peu ouvertes. Le terme faïençage n’est pas approprié pour la pierre : il décrit un réseau de fissures affectant un émail, un enduit."@en.
:_7285fd07 a skos:Concept;
           skos:inScheme :scheme;
           skos:prefLabel "Hair crack"@en;
           skos:prefLabel "Microfissure"@fr;
           skos:broader :_7eb0c1ad;
           skos:changeNote [
    dct:creator "Nicola Carboni";
    dct:modified "2017-05-24T16:10:01+00:00"
];
           skos:definition "Minor crack with width dimension < 0.1 mm"@en;
           skos:definition "Fissure d’ouverture inférieure à 0,1 mm."@fr.
:_94ebf59e a skos:Concept;
           skos:inScheme :scheme;
           skos:prefLabel "Splitting"@en;
           skos:prefLabel "Clivage"@fr;
           skos:broader :_7eb0c1ad;
           skos:changeNote [
    dct:creator "Nicola Carboni";
    dct:modified "2017-05-24T16:10:31+00:00"
];
           skos:definition "Fracturing of a stone along planes of weakness such as microcracks or clay/silt layers, in case where the structural elements are orientated vertically. For instance, a column may split into several parts along bedding planes if the load above it is too high."@en;
           skos:definition "Décrit le développement d’une cassure le long de plans de faiblesse tels que microfissures, couches argileuses, dans le cas où ces éléments structuraux sont orientés verticalement. Une pierre posée en délit, par exemple une colonne, peut se cliver le long des plans de litage si la charge qu’elle supporte est trop importante."@en.
:_bfe46976 a skos:Concept;
           skos:inScheme :scheme;
           skos:prefLabel "Star crack"@en;
           skos:prefLabel "Fissuration en ètoile"@fr;
           skos:broader :_7eb0c1ad;
           skos:changeNote [
    dct:creator "Nicola Carboni";
    dct:modified "2017-05-24T16:11:26+00:00"
];
           skos:definition "Crack having the form of a star. Rusting iron or mechanical impact are possible causes of this type of damage."@en;
           skos:definition "Ensemble de fissures se développant de façon rayonnante. La corrosion d’éléments métalliques, l’impact de projectiles sont des causes possibles de fissuration en étoile."@fr.
:_bb1ba8aa a skos:Concept;
           skos:inScheme :scheme;
           skos:prefLabel "Deformation"@en;
           skos:prefLabel "Déformation"@fr;
           skos:altLabel "Plastic deformation"@en;
           skos:altLabel "bowing"@en;
           skos:altLabel "Déformation plastique"@fr;
           skos:altLabel "distorsion"@fr;
           skos:altLabel "gauchissement"@fr;
           skos:broader :_72b9ad8d;
           skos:broader :_72b9ad8d;
           skos:definition "Change in shape without loosing integrity, leading to bending, buckling or twisting of a stone block."@en;
           skos:definition "Changement de forme conduisant à la courbure (convexe ou concave), au bombement ou à la torsion d’une pierre."@fr.
:_3b55e13d a skos:Concept;
           skos:topConceptOf :scheme;
           skos:inScheme :scheme;
           skos:prefLabel "Detachment"@en;
           skos:prefLabel "Détachement"@fr;
           skos:narrower :_482d9061;
           skos:narrower :_e2f202a8;
           skos:narrower :_e591da53;
           skos:narrower :_0975a0a5;
           skos:narrower :_d5038ac5;
           skos:narrower :_917b9098;
           skos:narrower :_d03d2c98.
:_482d9061 a skos:Concept;
           skos:inScheme :scheme;
           skos:prefLabel "Blistering"@en;
           skos:prefLabel "Boursouflure"@fr;
           skos:altLabel "Cloque"@fr;
           skos:broader :_3b55e13d;
           skos:definition "Separated, air-filled, raised hemispherical elevations on the face of stone resulting from the detachment of an outer stone layer. This detachment is not related to the stone structure"@en;
           skos:definition "Détachement d’une couche superficielle de la pierre sous forme d’un bombement creux plus ou moins fis- suré, et de forme sub-hémisphérique. Ce détachement est indépendant de la structure interne de la pierre."@en.
:_e2f202a8 a skos:Concept;
           skos:inScheme :scheme;
           skos:prefLabel "Bursting"@en;
           skos:prefLabel "Eclatement"@fr;
           skos:altLabel "Break out"@en;
           skos:broader :_3b55e13d;
           skos:definition "Local loss of the stone surface from internal pressure usually manifesting in the form of an irregularly-sided crater."@en;
           skos:definition "Perte locale de matière en surface de la pierre, due à des pressions internes, se manifestant habituellement sous la forme d’un cratère à bords irréguliers"@fr.
:_e591da53 a skos:Concept;
           skos:inScheme :scheme;
           skos:prefLabel "Delamination"@en;
           skos:prefLabel "Délitage"@fr;
           skos:altLabel "Layering"@en;
           skos:altLabel "Délamination"@fr;
           skos:altLabel "délitement"@fr;
           skos:broader :_3b55e13d;
           skos:narrower :_f870ad02;
           skos:definition "Detachment process affecting laminated stones (most of sedimentary rocks, some metamorphic rocks...). It corresponds to a physical separation into one or several layers following the stone laminae. The thickness and the shape of the layers are variable. The layers may be oriented in any direction with regards to the stone surface."@en;
           skos:definition "Détachement selon une orientation préexistante conduisant à la dissociation d’une ou quelques couches (lamines). Il affecte les pierres présentant un litage (pierres d’origine sédimentaire) ou des plans de schistosité (pierres d’origine métamorphique). L’épaisseur et la forme des couches sont variables."@fr.
:_f870ad02 a skos:Concept;
           skos:inScheme :scheme;
           skos:prefLabel "Exfoliation"@en;
           skos:prefLabel "Exfoliation"@fr;
           skos:broader :_e591da53;
           skos:definition "Detachment of multiple thin stone layers (cm scale) that are sub-parallel to the stone surface. The layers may bend, twist in a similar way as book pages."@en;
           skos:definition "Détachement de multiples couches, subparallèles à la surface de la pierre. Quand les couches détachées sont fines (épaisseur centimétrique), elles peuvent présenter des plis, des torsions, de la même façon que les pages gau- frées d’un livre."@en.
:_0975a0a5 a skos:Concept;
           skos:inScheme :scheme;
           skos:prefLabel "Disintegration"@en;
           skos:prefLabel "Désagrégation"@fr;
           skos:altLabel "Loss of cohesion"@en;
           skos:altLabel "incoherence"@en;
           skos:altLabel "decohesion"@en;
           skos:altLabel "friability"@en;
           skos:altLabel "disaggregation"@en;
           skos:altLabel "intergranular incoherence"@en;
           skos:altLabel "pulverization"@en;
           skos:altLabel "Décohésion"@fr;
           skos:altLabel "perte de cohésion"@fr;
           skos:altLabel "pulvérisation"@fr;
           skos:broader :_3b55e13d;
           skos:narrower :_db43170c;
           skos:narrower :_f734e949;
           skos:definition "It affects only the surface of the stone or can occur in depth. Damage generally starts from the surface of the material. On crystalline marble, granular disintegration may reach several centimeters in depth, sometimes more."@en;
           skos:definition "La désagrégation peut affecter la pierre en surface et/ou en profondeur. La dégradation commence généralement en sur- face. Dans le cas des marbres, elle peut atteindre plusieurs centimètres en profondeur, parfois plus."@fr.
:_db43170c a skos:Concept;
           skos:inScheme :scheme;
           skos:prefLabel "Crumbling"@en;
           skos:prefLabel "Emiettement"@fr;
           skos:altLabel "effritement"@fr;
           skos:broader :_0975a0a5;
           skos:changeNote [
    dct:creator "Nicola Carboni";
    dct:modified "2017-05-26T10:28:29+00:00"
];
           skos:definition "Detachment of aggregates of grains from the substrate. These aggregates are generally limited in size (less than 2 cm). This size depends of the nature of the stone and its environment."@en;
           skos:definition "Détachement d’agrégats de grains de pierre. Ces agrégats ont une taille géné- ralement inférieure à 2 cm, liée à la nature et à l’environne- ment de la pierre."@en.
:_f734e949 a skos:Concept;
           skos:inScheme :scheme;
           skos:prefLabel "Granular disintegration"@en;
           skos:prefLabel "Désagrégation granulaire"@fr;
           skos:broader :_0975a0a5;
           skos:narrower :_1a5fddd2;
           skos:narrower :_e78d7e33;
           skos:narrower :_db0eb19e;
           skos:definition "Occurs in granular sedimentary (e.g. sandstone) and granular crystalline (e.g. granite) stones. Granular disintegration produces debris referred to as a rock meal and can often be seen accumulating at the foot of wall actively deteriorating. If the stone surface forms a cavity (coving), the detached material may accumulate through gravity on the lower part of the cavity. The grain size of the stone determines the size of the resulting detached material. The following specific terms, all related to granular disintegration, refer either to the size, or to the aspect of corresponding grains :"@en;
           skos:definition "Se développe sur les roches granulaires (ex. grès) ou à texture grenue (ex. granites). Elle conduit souvent à la formation de dépôts meubles au dessous des zones affectées. Si la surface de la pierre forme une cavité (creusement), les matériaux détachés peuvent s’accumuler par gravité sur la partie inférieure de la cavité. La taille des grains détermine la taille des matériaux détachés"@fr.
:_1a5fddd2 a skos:Concept;
           skos:inScheme :scheme;
           skos:prefLabel "Powdering"@en;
           skos:prefLabel "Pulvérulence"@fr;
           skos:altLabel "Chalking"@en;
           skos:altLabel "Farinage"@fr;
           skos:broader :_f734e949;
           skos:definition "Term employed for describing granular disintegration of finely grained stones"@en;
           skos:definition "Désagrégation en poudre d’un matériau à grains fins (ex. craie)."@fr.
:_e78d7e33 a skos:Concept;
           skos:inScheme :scheme;
           skos:prefLabel "Sugaring"@en;
           skos:prefLabel "Désagrégation saccharoïde"@fr;
           skos:broader :_f734e949;
           skos:definition "Granular disintegration employed mainly in the white cristallyne marble domain"@en;
           skos:definition "Sous-types de désagrégation granulaire dans le domaine du marbres cristallins."@fr.
:_db0eb19e a skos:Concept;
           skos:inScheme :scheme;
           skos:prefLabel "Sanding"@en;
           skos:prefLabel "Désagrégation sableuse"@fr;
           skos:broader :_f734e949;
           skos:definition "Describe granular disintegration of sandstones and granites."@en;
           skos:definition "sous-types de désagrégation granulaire qui s’applique aux grès et aux granites."@fr.
:_d5038ac5 a skos:Concept;
           skos:inScheme :scheme;
           skos:prefLabel "Fragmentation"@en;
           skos:prefLabel "Fragmentation"@fr;
           skos:altLabel "Cassure"@fr;
           skos:broader :_3b55e13d;
           skos:narrower :_565e701c;
           skos:narrower :_63f6812c;
           skos:definition "The complete or partial breaking up of a stone, into portions of variable dimensions that are irregular in form, thickness and volume."@en;
           skos:definition "Fracturation partielle ou complète de la pierre en fragments de dimensions variables dont la forme, l’épaisseur et le volume sont irréguliers."@fr.
:_565e701c a skos:Concept;
           skos:inScheme :scheme;
           skos:prefLabel "Splintering"@en;
           skos:prefLabel "Fragmentation en esquilles"@fr;
           skos:broader :_d5038ac5;
           skos:definition "Detachment of sharp, slender pieces of stone, split or broken off from the main body."@en;
           skos:definition "Fracturation en un ou plu- sieurs fragments de forme allongée aux arêtes vives."@fr.
:_63f6812c a skos:Concept;
           skos:inScheme :scheme;
           skos:prefLabel "Chipping"@en;
           skos:prefLabel "Epaufrure"@fr;
           skos:broader :_d5038ac5;
           skos:definition "Breaking off of pieces, called chips, from the edges of a block."@en;
           skos:definition "Détachement d’un éclat sur une arête. Le frag-ment formé (chip en anglais) a une taille variable et une forme irrégulière."@en.
:_917b9098 a skos:Concept;
           skos:inScheme :scheme;
           skos:prefLabel "Peeling"@en;
           skos:prefLabel "Pelage"@fr;
           skos:altLabel "Peeling off"@en;
           skos:altLabel "Ecaillage"@fr;
           skos:broader :_3b55e13d;
           skos:changeNote [
    dct:creator "Nicola Carboni";
    dct:modified "2017-05-26T10:40:51+00:00"
];
           skos:changeNote [
    dct:creator "Nicola Carboni";
    dct:modified "2017-05-26T10:45:37+00:00"
];
           skos:definition "Shedding, coming off, or partial detachment of a superficial layer (thickness : submillimetric to millimetric) having the aspect of a film or coating which has been applied on the stone surface."@en;
           skos:definition "Décollement partiel ou total d’une fine couche (épaisseur inframillimétrique à millimétrique) ayant l’aspect d’un film ou d’un revêtement appliqué sur la pierre."@fr;
           skos:scopeNote """Not to be confused with :
- Blistering, which is associated with a dome-like morphology. 
- Scaling, which is related to the detachment of stone layers (thickness : millimetric to centimetric)."""@en;
           skos:scopeNote """Ne pas confondre avec :
- Boursouflure, associé à une forme en dôme.
- Desquamation, qui se rapporte au détachement de couches de pierre d’épaisseur millimétrique à centimétrique."""@fr.
:_d03d2c98 a skos:Concept;
           skos:inScheme :scheme;
           skos:prefLabel "Scaling"@en;
           skos:prefLabel "Desquamation"@fr;
           skos:broader :_3b55e13d;
           skos:definition "Detachment of stone as a scale or a stack of scales, not following any stone structure and detaching like fish scales or parallel to the stone surface. The thickness of a scale is generally of millimetric to centimetric scale, and is negligeable compared to its surface dimension."@en;
           skos:definition """Détachement d’écailles de pierre individuelles ou en paquets indépendamment de toute structure orientée préexistante. La desquamation se développe parallèlement à la surface ou en écailles de poisson. L’épaisseur des écailles est négligeable par rapport à leur extension.
"""@fr;
           skos:scopeNote """Not to be confused with :
- Delamination : corresponds to a detachment following the bedding or shistosity planes of a stone."""@en;
           skos:scopeNote """Ne pas confondre avec :
- Délitage : correspond à un détachement selon une orientation préexistante, telle que des plans de litage ou des plans de schistosité."""@en.
:_1b1b0219 a skos:Concept;
           skos:topConceptOf :scheme;
           skos:inScheme :scheme;
           skos:prefLabel "Features Induced by Material Loss"@en;
           skos:prefLabel "Figures Induites Par Une Perte De matière"@fr;
           skos:narrower :_acd059a1;
           skos:narrower :_d3a7418f;
           skos:narrower :_7e6e3e54;
           skos:narrower :_bd2e89b5;
           skos:narrower :_30ee47a5;
           skos:narrower :_2156999c;
           skos:narrower :_138a67a5.
:_acd059a1 a skos:Concept;
           skos:inScheme :scheme;
           skos:prefLabel "Alveolization"@en;
           skos:prefLabel "Alvéolisation"@fr;
           skos:altLabel "Alveolar erosion"@en;
           skos:altLabel "alveolar weathering"@en;
           skos:altLabel "honeycomb"@en;
           skos:altLabel "Alveolisation"@en;
           skos:broader :_1b1b0219;
           skos:narrower :_509b2e09;
           skos:definition "Formation, on the stone surface, of cavities (alveoles) which may be interconnected and may have variable shapes and sizes (generally centimetric, sometimes metric)."@en;
           skos:definition "Formation, à la surface de la pierre, de cavités (alvéoles) variables en forme et taille (souvent centimétrique, parfois métrique), et qui peuvent être interconnectées."@fr;
           skos:scopeNote """Not to be confused with :
- Microkarst : refers to a network of millimetric to centrimetric interconnected depressions, clearly linked to a dissolution pro- cess.
- Pitting : corresponds to the formation of point-like millime- tric to submillimetric pits, generally not connected, on a stone surface."""@en;
           skos:scopeNote """Ne pas confondre avec :
- Microkarst : se rapporte à un réseau de cavités manifestement dues à une dissolution, et qui confèrent un aspect raviné à la surface de la pierre.
- Pitting : correspond à la formation de microcavités généralement non connectées."""@fr.
:_509b2e09 a skos:Concept;
           skos:inScheme :scheme;
           skos:prefLabel "Coving"@en;
           skos:prefLabel "Creusement"@fr;
           skos:broader :_acd059a1;
           skos:definition "Erosion feature consisting in a single alveole developing from the edge of the stone block."@en;
           skos:definition "S’applique à la formation d’une seule alvéole affectant la surface de la pierre à partir de ses arêtes."@fr.
:_d3a7418f a skos:Concept;
           skos:inScheme :scheme;
           skos:prefLabel "Erosion"@en;
           skos:prefLabel "Érosion"@fr;
           skos:altLabel "Loss of material"@en;
           skos:broader :_1b1b0219;
           skos:narrower :_e0214972;
           skos:narrower :_bd3685d7;
           skos:narrower :_d6367d5a;
           skos:definition "Loss of original surface, leading to smoothed shapes."@en;
           skos:definition "Disparition de la surface originelle de la pierre, conduisant à des contours émoussés."@fr.
:_e0214972 a skos:Concept;
           skos:inScheme :scheme;
           skos:prefLabel "Differential erosion"@en;
           skos:prefLabel "Érosion différentielle"@fr;
           skos:altLabel "Differential deterioration"@en;
           skos:altLabel "Relief formation"@en;
           skos:broader :_d3a7418f;
           skos:narrower :_d076f3dd;
           skos:narrower :_734879f0;
           skos:definition "occurs when erosion does not proceed at the same rate from one area of the stone to the other. As a result, the stone deteriorates irregularly. This feature is found on heterogeneous stones containing harder and/or less porous zones. It may also occur as a result of selective lichen attack on calci- tic stones. Differential erosion is generally found on sedimentary and volcanic stones"@en;
           skos:definition "Conduit à la formation de reliefs, par exemple à la création d’irrégularités à la surface de la pierre. Elle apparaît si l’érosion ne progresse pas de façon homogène sur toute la surface de la pierre. On trouve cette figure sur les pierres hétérogènes, contenant des zones plus dures et/ou moins poreuses. Les roches calcitiques peuvent aussi présenter une érosion différentielle résultant d’une attaque sélective par des lichens. Certaines roches sédimen- taires et volcaniques sont particulièrement sujettes à ce type d’altération."@en.
:_d076f3dd a skos:Concept;
           skos:inScheme :scheme;
           skos:prefLabel "Loss of components"@en;
           skos:prefLabel "Perte de constituants"@fr;
           skos:broader :_e0214972;
           skos:definition "Partial or selective elimination of soft or compact stone components "@en;
           skos:definition "Correspond à l’élimination sélective de constituants plus tendres  ou plus compacts."@en;
           skos:example "lentilles d’argile, nodules de limonite,  galets, fragments de fossiles, concrétions"@fr;
           skos:example "clay lenticles, nodes of limonite, pebbles, fossil fragments, geological concretions, lava fragments"@en.
:_734879f0 a skos:Concept;
           skos:inScheme :scheme;
           skos:prefLabel "Loss of matrix"@en;
           skos:prefLabel "Perte de matrice"@fr;
           skos:broader :_e0214972;
           skos:definition "Partial or selective elimination of the stone matrix, resulting in protruding compact stone components."@en;
           skos:definition "Processus inverse correspondant à une élimination sélective de la matrice de la pierre, avec pour conséquence la mise en relief de constituants compacts de la pierre"@fr;
           skos:example "galets, fossiles, fragments de lave"@fr.
:_bd3685d7 a skos:Concept;
           skos:inScheme :scheme;
           skos:prefLabel "Rounding"@en;
           skos:prefLabel "Erosion en boule"@fr;
           skos:broader :_d3a7418f;
           skos:definition "Preferential erosion of originally angular stone edges leading to a distinctly rounded profile. Rounding can especially be observed on stones which preferably deteriorate through granular disintegration, or when environmental conditions favor granular disintegration."@en;
           skos:definition "Forme arrondie résultant de l’érosion préférentielle des bords originellement anguleux d’une pierre. On observe cette forme d’altération sur les pierres sujettes à la désagrégation granulaire, ou placées dans des conditions telles que la désagrégation granulaire peut se développer."@fr.
:_d6367d5a a skos:Concept;
           skos:inScheme :scheme;
           skos:prefLabel "Roughening"@en;
           skos:prefLabel "Augmentation de rugosité"@fr;
           skos:broader :_d3a7418f;
           skos:definition "Selective loss of small particles from an ori- ginally smooth stone surface. The substrate is still sound. Roughening can appear either progressively in case of long term deterioration process (for instance in case of granular disintegration), or instantaneously in case of inappropriate actions, such as aggressive cleaning."@en;
           skos:definition "correspond à un accroissement de rugosité d’une surface originellement douce, par perte sélective de petites particules sur un substrat encore sain. Dans le cas d’une pierre originellement polie, on parle dépolissage. Une augmentation de rugosité peut être progressive car due à une exposition continue aux agents de détério- ration, (exemple : désagrégation granulaire) ou immédiate, comme lors d’un nettoyage agressif."@en.
:_7e6e3e54 a skos:Concept;
           skos:inScheme :scheme;
           skos:prefLabel "Mechanical Damage"@en;
           skos:prefLabel "Dégât mécanique"@fr;
           skos:altLabel "Arrachement"@fr;
           skos:broader :_1b1b0219;
           skos:narrower :_35ec0223;
           skos:narrower :_efca5af7;
           skos:narrower :_b9b1a07e;
           skos:narrower :_80dda7ce;
           skos:narrower :_8245c84c;
           skos:definition "Loss of stone material clearly due to a mechanical action."@en;
           skos:definition "Perte de matière due à une action mécanique."@fr.
:_35ec0223 a skos:Concept;
           skos:inScheme :scheme;
           skos:prefLabel "Impact damage"@en;
           skos:prefLabel "Trace d’impact"@fr;
           skos:broader :_7e6e3e54;
           skos:definition "Mechanical damage due to the impact of a projectile (bullet, shrapnel) or of a hard tool."@en;
           skos:definition "Dégât mécanique dû à l’impact d’un projectile (balle, éclat d’obus etc.) ou d’un outil dur."@fr.
:_efca5af7 a skos:Concept;
           skos:inScheme :scheme;
           skos:prefLabel "Cut"@en;
           skos:prefLabel "Incision"@fr;
           skos:broader :_7e6e3e54;
           skos:definition "Loss of material due to the action of an edge tool. It can have the appearance of an excavated cavity, an incision, a missing edge, etc...Tool marks can be considered as special kinds of cuts but should not be considered as damage features."@en;
           skos:definition "Marque laissée par l’élimination de matière à l’aide d’un instrument coupant. Une incision peut avoir l’apparence d’une cavité excavée, une coupure, un bord manquant, etc. Les marques d’outil peuvent être considérées comme des formes spéciales d’incisions, mais ne devraient pas être consi- dérées comme des formes d’altération. Certains graffitis peuvent être faits par incision de la pierre."@fr.
:_b9b1a07e a skos:Concept;
           skos:inScheme :scheme;
           skos:prefLabel "Scratch"@en;
           skos:prefLabel "Rayure"@fr;
           skos:altLabel "éraflure"@fr;
           skos:broader :_7e6e3e54;
           skos:definition "Manually induced superficial and line-like loss of material due to the action of some pointed object. It can be accidental or intentional. Usually it appears as a more or less long groove. Tool marks can have the appearance of scratches, but should not be taken as damage features"@en;
           skos:definition "Perte linéaire de matière, accidentelle ou intentionnelle, provoquée par l’action manuelle d’un objet pointu. Habituellement, les rayures apparaissent sous forme de sillons plus ou moins longs, isolés ou associés en séries. Les outils de taille peuvent laisser des traces ayant l’ap- parence de rayures, mais ces traces ne doivent pas être consi- dérées comme des signes d’altération. La griffure (ex. de pigeon) est une forme de rayure."@en.
:_80dda7ce a skos:Concept;
           skos:inScheme :scheme;
           skos:prefLabel "Abrasion"@en;
           skos:prefLabel "Abrasion"@fr;
           skos:broader :_7e6e3e54;
           skos:definition "Erosion due to wearing down or rubbing away by means of friction, or to the impact of particles."@en;
           skos:definition "Erosion due à un frottement (attrition) ou à l’impact de particules."@fr.
:_8245c84c a skos:Concept;
           skos:inScheme :scheme;
           skos:prefLabel "Keying"@en;
           skos:prefLabel "Bûchage"@fr;
           skos:broader :_7e6e3e54;
           skos:definition "Impact damage resulting from hitting a surface with a pointed tool, in order to get an irregular surface which will assist the adhesion of an added material, a mortar for instance."@en;
           skos:definition "Ensemble d’entailles réalisées par un outil de taille. Ces entailles ont pour but de rendre la surface irrégulière de façon à favoriser l’accrochage mécanique d’un matériau rajouté, un mortier par exemple. Le bûchage désigne aussi en Français l’élimination, par vandalisme, d’une partie saillante d’une sculpture."@en.
:_bd2e89b5 a skos:Concept;
           skos:inScheme :scheme;
           skos:prefLabel "Microkarst"@en;
           skos:prefLabel "Microkarst"@fr;
           skos:altLabel "Karst"@en;
           skos:altLabel "dissolution"@en;
           skos:altLabel "cratering"@en;
           skos:altLabel "Karst"@fr;
           skos:broader :_1b1b0219;
           skos:definition "Network of small interconnected depressions of millimetric to centrimetric scale, sometimes looking like hydrographic network. Microkarst patterns are due to a partial and/or selective dissolution of calcareous stone surfaces exposed to water run-off."@en;
           skos:definition "Réseau de petites dépressions interconnectées, d’é- chelle millimétrique à centimétrique, ayant parfois l’aspect d’un réseau hydrographique. Généralement, les figures de microkarst sont dues à une dissolution partielle ou sélective de la surface des pierres cal- caires exposées au ruissellement d’eau."@fr.
:_30ee47a5 a skos:Concept;
           skos:inScheme :scheme;
           skos:prefLabel "Missing Part"@en;
           skos:prefLabel "Partie Manquante"@fr;
           skos:altLabel "Lacuna"@en;
           skos:altLabel "Manque"@fr;
           skos:altLabel "lacune"@fr;
           skos:broader :_1b1b0219;
           skos:narrower :_adc1f652;
           skos:changeNote [
    dct:creator "Nicola Carboni";
    dct:modified "2017-05-26T11:53:40+00:00"
];
           skos:definition "Empty space, obviously located in the place of some formerly existing stone part. Protruding and particularly exposed parts of sculptures (nose, fingers..) are typical locations for material loss resulting in missing parts."@en;
           skos:definition "Absence de tout ou partie d’une pierre. Cette figure d’altération affecte fréquemment les éléments pro- éminents et particulièrement exposés des sculptures (nez, orteils, doigts)."@fr.
:_adc1f652 a skos:Concept;
           skos:inScheme :scheme;
           skos:prefLabel "Gap"@en;
           skos:prefLabel "Trou"@fr;
           skos:broader :_30ee47a5;
           skos:definition "Hollow place in the stone surface, hole."@en;
           skos:definition "Espace vide, cavité."@fr.
:_2156999c a skos:Concept;
           skos:inScheme :scheme;
           skos:prefLabel "Perforation"@en;
           skos:prefLabel "Perforation"@fr;
           skos:altLabel "Drill hole"@en;
           skos:altLabel "Percement"@fr;
           skos:broader :_1b1b0219;
           skos:definition "A single or series of surface punctures, holes or gaps, made by a sharp tool or created by an animal. The size is generally of millimetric to centrimetric scale. Perforations are deeper than wide, and penetrate into the body of the stone"@en;
           skos:definition "Poinçonnement, percement, simple ou multiple, de taille milli- à centimétrique, induit par un animal ou un outil, qui s’étend en profondeur. Une perforation est plus profonde que large."@en.
:_138a67a5 a skos:Concept;
           skos:inScheme :scheme;
           skos:prefLabel "Pitting"@en;
           skos:prefLabel "Pitting"@fr;
           skos:altLabel "Piqûre"@fr;
           skos:broader :_1b1b0219;
           skos:definition "Point-like millimetric or submillimetric shallow cavities. The pits generally have a cylindrical or conical shape and are not interconnected, although transitions patterns to interconnected pits can also be observed."@en;
           skos:definition "Cavité millimétrique ou submillimétrique peu profonde. Les piqûres ont généralement une forme conique ou cylindrique et ne sont pas connectées. On peut observer cependant des formes de transition vers un système de piqûres interconnectées."@en.
:_5a84d36f a skos:Concept;
           skos:topConceptOf :scheme;
           skos:inScheme :scheme;
           skos:prefLabel "Discoloration & Deposit"@en;
           skos:prefLabel "Altération Chromatique Et Dépôt"@fr;
           skos:narrower :_aef6e65f;
           skos:narrower :_b97947cd;
           skos:narrower :_9f0dbe68;
           skos:narrower :_df535bef;
           skos:narrower :_cd96d942;
           skos:narrower :_6f81e9f4;
           skos:narrower :_ca92d3de;
           skos:narrower :_18cf420d;
           skos:narrower :_c5d14f6e;
           skos:narrower :_6f196125;
           skos:narrower :_f2f9010b.
:_aef6e65f a skos:Concept;
           skos:inScheme :scheme;
           skos:prefLabel "Crust"@en;
           skos:prefLabel "Croûte"@fr;
           skos:broader :_5a84d36f;
           skos:narrower :_b585fe2d;
           skos:narrower :_d6e58167;
           skos:definition "Generally coherent accumulation of materials on the surface. A crust may include exogenic deposits in combination with materials derived from the stone. A crust is frequently dark coloured (black crust) but light colours can also be found. Crusts may have an homogeneous thickness, and thus replicate the stone surface, or have irregular thickness and disturb the reading of the stone surface details."@en;
           skos:definition "Accumulation de matériaux en une ou plusieurs couches superficielles cohérentes. Une croûte peut contenir des dépôts exogènes combinés avec des matériaux dérivés de la pierre. Une croûte est fréquemment de couleur foncée (ex. Croûte noire) mais on rencontre aussi des croûtes de teinte claire. Les croûtes peuvent avoir une épaisseur homogène, auquel cas elles reproduisent fidèlement les contours de la pierre, ou bien avoir une épaisseur irrégulière ce qui perturbe la lecture des détails superficiels."@en.
:_b585fe2d a skos:Concept;
           skos:inScheme :scheme;
           skos:prefLabel "Black crust"@en;
           skos:prefLabel "Croûte noire"@fr;
           skos:broader :_aef6e65f;
           skos:definition "Kind of crust developing generally on areas protected against direct rainfall or water runoff in urban envi- ronment. Black crusts usually adhere firmly to the substrate. They are composed mainly of particles from the atmosphere, trapped into a gypsum (CaSO4.2H2O). matrix."@en;
           skos:definition "Croûte de couleur grise à noire, habituelle- ment fortement adhérente, et qui se développe en milieu urbain, dans des zones protégées de l’impact direct de la pluie ou des ruissellements d’eau. Les croûtes noires sont principalement constituées de particules provenant de l’atmosphère, piégées dans une matrice de gypse (CaSO4.2H2O)."@en.
:_d6e58167 a skos:Concept;
           skos:inScheme :scheme;
           skos:prefLabel "Salt crust"@en;
           skos:prefLabel "Croûte saline"@fr;
           skos:broader :_aef6e65f;
           skos:definition "Crust composed of soluble salts, which develop in the presence of high salt levels, and form from wetting and drying cycles."@en;
           skos:definition "Croûte composée de sels solubles, qui se développe dans un contexte de forte teneur en sel, au gré des cycles d’humectation-dessiccation."@fr.
:_b97947cd a skos:Concept;
           skos:inScheme :scheme;
           skos:prefLabel "Deposit"@en;
           skos:prefLabel "Dépôt"@fr;
           skos:altLabel "Dépôt superficiel"@en;
           skos:altLabel "Surface deposit"@fr;
           skos:broader :_5a84d36f;
           skos:definition "Accumulation of exogenic material of variable thickness. Some examples of deposits : splashes of paint or mortar, sea salt aerosols, atmospheric particles such as soot or dust, remains of conservation materials such as cellulose poultices, blast materials etc.."@en;
           skos:definition "Accumulation superficielle de matériaux exogènes formant une couche peu cohérente et d’épaisseur variable. Exemples de dépôts : éclaboussures de peinture ou de mortier, sels provenant d’aérosols marins, poussières, restes de matériaux de conservation comme compresses cellulosiques, poudres de sablage etc."@fr.
:_9f0dbe68 a skos:Concept;
           skos:inScheme :scheme;
           skos:prefLabel "Discolouration"@en;
           skos:prefLabel "Altération Chromatique"@fr;
           skos:altLabel "Chromatic alteration"@en;
           skos:altLabel "Discoloration"@en;
           skos:broader :_5a84d36f;
           skos:narrower :_6628bd65;
           skos:narrower :_838f6f3f;
           skos:narrower :_99212a6c;
           skos:narrower :_b62a3e2f;
           skos:changeNote [
    dct:creator "Nicola Carboni";
    dct:modified "2017-05-26T12:04:22+00:00"
];
           skos:definition """Change of the stone colour in one to three of the colour parameters : hue, value and chroma.
- hue corresponds to the most prominent characte- ristic of a colour (blue, red, yellow, orange etc..).
- value corresponds to the darkness (low hues) or lightness (high hues) of a colour.
- chroma corresponds to the purity of a colour. High chroma colours look rich and full. Low chroma colours look dull and grayish. Sometimes chroma is called saturation."""@en;
           skos:definition """Modification d’un ou plusieurs des paramètres caracté- risant la couleur de la pierre : teinte, clarté, saturation. Teinte : correspond à la caractéristique la plus mar- quante de la couleur (bleu, rouge, jaune, orange etc.). Clarté : correspond au caractère foncé (clarté fai- ble), ou clair (forte clarté) de la couleur.
Saturation : correspond à la pureté d’une couleur. Les couleurs à saturation élevée paraissent vives et pleines. Les couleurs à saturation faible paraissent grisâtres et ternes."""@fr.
:_6628bd65 a skos:Concept;
           skos:inScheme :scheme;
           skos:prefLabel "Colouration"@en;
           skos:prefLabel "Coloration"@fr;
           skos:altLabel "colouring"@en;
           skos:broader :_9f0dbe68;
           skos:definition "Change in hue, value and/or a gain in chroma"@en;
           skos:definition "Changement de teinte, de clarté et /ou à un gain en saturation."@en.
:_838f6f3f a skos:Concept;
           skos:inScheme :scheme;
           skos:prefLabel "Bleaching"@en;
           skos:prefLabel "Décoloration"@fr;
           skos:altLabel "fading"@en;
           skos:broader :_9f0dbe68;
           skos:definition "gain in value due to chemical weathering of minerals (e.g. reduction of iron and manganese compounds) or extraction of coloring matter (leaching, was- hing out), or loss of polish, generally very superficial. Dark and bright color marbles often show bleaching as a result of exposure to weather."@en;
           skos:definition "augmentation de clarté, due à l’altération chimique des minéraux (par exemple réduction du fer et du manganèse) ou à l’extraction de matière colorante (par lavage, lessivage), ou par perte de poli, généralement très superficielle. Les marbres foncés et ceux de couleurs vives subissent souvent une décoloration suite à une exposition aux intempéries. Un blanchiment est une sorte de décoloration."@en.
:_99212a6c a skos:Concept;
           skos:inScheme :scheme;
           skos:prefLabel "Moist area"@en;
           skos:prefLabel "Assombrissement du à l’humidité"@fr;
           skos:altLabel "moist spot"@en;
           skos:altLabel "moist zone or visible damp area"@en;
           skos:altLabel "tache d’humidité"@fr;
           skos:altLabel "zone humide visible"@fr;
           skos:broader :_9f0dbe68;
           skos:definition "Corresponds to the darkening (lower hue) of a surface due to dampness"@en;
           skos:definition "Assombrissement du à l’humidité est considérée comme une altération chromatique (baisse de saturation)."@en.
:_b62a3e2f a skos:Concept;
           skos:inScheme :scheme;
           skos:prefLabel "Staining"@en;
           skos:prefLabel "Tache"@fr;
           skos:broader :_9f0dbe68;
           skos:definition "Kind of discolouration of limited extent and generally of unattractive appearance."@en;
           skos:definition ">one d’extension limitée présentant une altération chromatique et ayant une apparence déplaisante."@en.
:_df535bef a skos:Concept;
           skos:inScheme :scheme;
           skos:prefLabel "Efflorescence"@en;
           skos:prefLabel "Efflorescence"@fr;
           skos:altLabel "loose salt deposits"@en;
           skos:altLabel "Efflorescence saline"@fr;
           skos:altLabel "salpêtre"@fr;
           skos:broader :_5a84d36f;
           skos:definition "Generally whitish, powdery or whisker-like crystals on the surface. Efflorescences are generally poorly cohesive and commonly made of soluble salt crystals."@en;
           skos:definition "Amas de cristaux habituellement blancs, d’aspect poudreux, aciculaire (en forme d’aiguilles) ou filamenteux, localisés en surface de la pierre. En général, les efflorescences sont peu cohérentes et constituées de sels solubles."@fr.
:_cd96d942 a skos:Concept;
           skos:inScheme :scheme;
           skos:prefLabel "Encrustation"@en;
           skos:prefLabel "Encroûtement"@fr;
           skos:altLabel "Incrustation"@en;
           skos:broader :_5a84d36f;
           skos:narrower :_643a3a6b;
           skos:definition "Compact, hard, mineral outer layer adhering to the stone. Surface morphology and colour are usually different from those of the stone."@en;
           skos:definition "Couche superficielle compacte, dure et adhérente. La morphologie superficielle et la couleur sont habituellement différentes de celles de la pierre."@en.
:_643a3a6b a skos:Concept;
           skos:inScheme :scheme;
           skos:prefLabel "Concretion"@en;
           skos:prefLabel "Concrétion"@fr;
           skos:broader :_cd96d942;
           skos:definition "Kind of encrustation having a specific shape: nodular, botryoïdal (grape-like) or framboïdal (raspberry like). Concretions may even have conic shapes of form drapery-like vertical sheets. Stalagmites and stalactites are kinds of concretions. In general, concretions do not outline, contour the surface of the stone, and are of limited extent."@en;
           skos:definition "Sorte d’encroûtement en forme de dépôt compact noduleux, botryoïde (comme une grappe) ou framboïde (comme une framboise). Une concrétion peut même avoir des formes coniques ou constituer des feuillets verticaux (draperies). Les stalagmites et stalactites sont des sortes de concrétions. En général, les concrétions ont une épaisseur irrégulière et ne suivent pas les contours des pierres. Elles ont une extension latérale limitée."@en.
:_6f81e9f4 a skos:Concept;
           skos:inScheme :scheme;
           skos:prefLabel "Film"@en;
           skos:prefLabel "Film"@fr;
           skos:altLabel "Pellicle"@en;
           skos:altLabel "skin"@en;
           skos:altLabel "Pellicule"@fr;
           skos:altLabel "peau"@fr;
           skos:broader :_5a84d36f;
           skos:definition "Thin covering or coating layer generally of organic nature, generally homogeneous, follows the stone surface. A film may be opaque or translucent"@en;
           skos:definition "Recouvrement mince, homogène, d’épaisseur généralement uniforme, habituellement de nature organique, souvent transparent, et qui épouse la surface de la pierre."@en.
:_ca92d3de a skos:Concept;
           skos:inScheme :scheme;
           skos:prefLabel "Glossy Aspect"@en;
           skos:prefLabel "Aspect Luisant"@fr;
           skos:altLabel "Polished surface"@en;
           skos:broader :_5a84d36f;
           skos:definition "Aspect of a surface that reflects totally or partially the light. The surface has a mirror-like appearance."@en;
           skos:definition "Aspect de surface qui reflète totalement ou partiellement la lumière. La surface ressemble à un miroir."@fr.
:_18cf420d a skos:Concept;
           skos:inScheme :scheme;
           skos:prefLabel "Graffiti"@en;
           skos:prefLabel "Graffiti"@fr;
           skos:altLabel "Graffitis"@en;
           skos:broader :_5a84d36f;
           skos:definition "Engraving, scratching, cutting or application of paint, ink or similar matter on the stone surface."@en;
           skos:definition "Forme d’altération superficielle résultant d’une incision, rayure ou application de peinture, encre ou matériau assimilé."@en.
:_c5d14f6e a skos:Concept;
           skos:inScheme :scheme;
           skos:prefLabel "Patina"@en;
           skos:prefLabel "Patine"@fr;
           skos:broader :_5a84d36f;
           skos:narrower :_4572340a;
           skos:narrower :_8bcd2576;
           skos:definition "Chromatic modification of the material, generally resulting from natural or artificial ageing and not involving in most cases visible surface deterioration."@en;
           skos:definition "Modification chromatique superficielle, résultant d’une altération naturelle ou artificielle et n`impliquant généralement pas de dégradation superficielle visible."@en.
:_4572340a a skos:Concept;
           skos:inScheme :scheme;
           skos:prefLabel "Iron rich patina"@en;
           skos:broader :_c5d14f6e;
           skos:definition "Natural black to brown thin layer enriched in iron/clay minerals, which can be found on iron containing sandstones. This kind of patina is generally observed in outdoors environment, and develops quite uniformly on the stone surface."@en;
           skos:definition "Type de patine brune à noire, se formant naturellement sur les grès contenant du fer. Elles se développent assez uniformément sur la surface de la pierre, dans les zones exposées aux intempéries."@fr.
:_8bcd2576 a skos:Concept;
           skos:inScheme :scheme;
           skos:prefLabel "Oxalate patina"@en;
           skos:prefLabel "Patine d’oxalates"@fr;
           skos:broader :_c5d14f6e;
           skos:definition "Orange to brown thin layer enriched in calcium oxalates. This kind of patina may be found in outdoors environment, often on marble and limestone substrates."@en;
           skos:definition "Ces patines, orange à brunes, sont de fines couches enrichies en oxalates de calcium. Elles se forment sur différents substrats, le plus souvent sur calcaires et marbres, en milieu extérieur."@fr.
:_6f196125 a skos:Concept;
           skos:inScheme :scheme;
           skos:prefLabel "Soiling"@en;
           skos:prefLabel "Encrassement"@fr;
           skos:altLabel "Salissure"@fr;
           skos:broader :_5a84d36f;
           skos:definition "Deposit of a very thin layer of exogenous particles (eg. soot) giving a dirty appearance to the stone surface."@en;
           skos:definition "Dépôt très fin de particules exogènes (par ex. poussières, suies) donnant un aspect sale à la surface de pierre"@en.
:_f2f9010b a skos:Concept;
           skos:inScheme :scheme;
           skos:prefLabel "Subflorescence"@en;
           skos:prefLabel "Subflorescence"@fr;
           skos:altLabel "Cryptoflorescence"@en;
           skos:altLabel "Cryptoflorescence"@fr;
           skos:broader :_5a84d36f;
           skos:definition "Poorly adhesive soluble salts, commonly white, located under the stone surface."@en;
           skos:definition "Cristaux de sels habituellement blancs, peu adhérents, formés sous la surface de la pierre."@fr.
:_26134f96 a skos:Concept;
           skos:inScheme :scheme;
           skos:prefLabel "Biological Colonization"@en;
           skos:prefLabel "Colonisation Biologique"@fr;
           skos:altLabel "Biological growth"@en;
           skos:altLabel "biological overgrowth"@en;
           skos:altLabel "living exogenous material"@en;
           skos:altLabel "Biological colonisation"@en;
           skos:altLabel "Croissance biologique"@fr;
           skos:altLabel "Prolifération végétale"@fr;
           skos:broader :_94af0e38;
           skos:definition "Colonization of the stone by plants and micro-organisms such as bacteria, cyanobacteria, algae, fungi and lichen (symbioses of the latter three). Biological colonization also includes influences by other organisms such as animals nesting on and in stone."@en;
           skos:definition "L’expression colonisation biologique s’applique surtout aux plantes et aux microorganismes tels que bactéries, cyanobactéries, algues, moisissures et lichens (symbioses des trois derniers). Il s’applique aussi aux structures fabriquées par des animaux, tels que des nids."@en.
:_94af0e38 a skos:Concept;
           skos:topConceptOf :scheme;
           skos:inScheme :scheme;
           skos:prefLabel "Biological Colonizations"@en;
           skos:prefLabel "Colonisations Biologiques"@fr;
           skos:narrower :_26134f96;
           skos:narrower :_f81d9f94;
           skos:narrower :_8c7c6043;
           skos:narrower :_dddfe749;
           skos:narrower :_b67fd3d4;
           skos:narrower :_6bb28298;
           skos:changeNote [
    dct:creator "Nicola Carboni";
    dct:modified "2017-05-26T13:54:57+00:00"
].
:_f81d9f94 a skos:Concept;
           skos:inScheme :scheme;
           skos:prefLabel "Alga"@en;
           skos:prefLabel "Algue"@fr;
           skos:altLabel "algae"@en;
           skos:broader :_94af0e38;
           skos:definition "Algae are microscopic vegetal organisms without stem nor leaves which can be seen outdoors and indoors, as powdery or viscous deposits (thickness : tenth of mm to several mm). Algae form green, red, brown, or black veil like zones and can be found mainly in situations where the substrate remains moistened for long periods of time. Depending on the environmental conditions and substrate type, algae may form solid layers or smooth films. On monuments, algae are constituted of unicellular to pluricellular clusters, and they never form macro- organisms."@en;
           skos:definition """Les algues sont des organismes végétaux microscopiques sans tige ni feuille formant à l’intérieur comme à l’extérieur des édifices des voiles verts, noirs ou rouges ou bruns (épaisseur quelques dixièmes de mm à plusieurs mm). Selon les conditions environnementales et le substrat les algues peuvent former des films pulvérulents ou visqueux. Les algues se développent principalement dans les situations où la surface du substrat reste humide pendant de longues périodes. Sur les monuments, les algues sont constituées de rassemblements uni-ou multicellulaires, elles ne forment jamais de macro-organismes.
"""@en.
:_8c7c6043 a skos:Concept;
           skos:inScheme :scheme;
           skos:prefLabel "Lichen"@en;
           skos:prefLabel "Lichen"@fr;
           skos:broader :_94af0e38;
           skos:narrower :_29e4d8d0;
           skos:narrower :_9963b31d;
           skos:narrower :_3debb2ac;
           skos:definition "Vegetal organism forming rounded millimetric to centimetric crusty or bushy patches, often having a leathery appearence, growing generally on outside parts of a building. Lichen are most commonly grey, yellow, orange, green or black and show no differentiation into stem, root and leaf."@en;
           skos:definition "Structure végétale millimétrique à centimétrique, généralement arrondie, ayant un aspect encroûtant ou buissonnant, et l’aspect du cuir. De couleur variée (orange, vert, gris, brun ou noir), ils ne montrent pas de différenciation en feuilles, tige et racine. Les lichens se développent généralement sur les surfaces externes de monuments."@en.
:_29e4d8d0 a skos:Concept;
           skos:inScheme :scheme;
           skos:prefLabel "Crustose lichen"@en;
           skos:prefLabel "Lichen encroûtant"@fr;
           skos:broader :_8c7c6043.
:_9963b31d a skos:Concept;
           skos:inScheme :scheme;
           skos:prefLabel "Folious lichen"@en;
           skos:prefLabel "Lichen foliacé"@fr;
           skos:broader :_8c7c6043.
:_3debb2ac a skos:Concept;
           skos:inScheme :scheme;
           skos:prefLabel "Epilithic lichen"@en;
           skos:prefLabel "Lichen épilithique"@fr;
           skos:broader :_8c7c6043.
:_dddfe749 a skos:Concept;
           skos:inScheme :scheme;
           skos:prefLabel "Moss"@en;
           skos:prefLabel "Mousse"@fr;
           skos:broader :_94af0e38;
           skos:definition """
Vegetal organism forming small, soft and green cushions of centimetric size. Mosses look generally like dense micro-leaves (sub- to millimetric size) tightly packed together. Mosses often grow on stone surface open cavities, cracks, and in any place permanently or frequently wet (masonry joints), and usually shady."""@en;
           skos:definition "Organisme végétal en forme de coussinets verts souples au toucher, de taille centimétrique. Les mousses ont l’apparence de petites feuilles (taille submillimétrique à millimétrique) assemblées en bouquets serrés. Les mousses se développent dans des cavités ouvertes, des fissures, des joints, toutes zones constamment ou souvent humides et/ou ombragées"@fr.
:_b67fd3d4 a skos:Concept;
           skos:inScheme :scheme;
           skos:prefLabel "Mould"@en;
           skos:prefLabel "Moisissure"@fr;
           skos:altLabel "Fungi"@en;
           skos:altLabel "Mold"@en;
           skos:broader :_94af0e38;
           skos:definition "Microscopic fungus which colonies, to the naked eye, look like a downy film or a network or star-like millimetric patches of filaments of diverse colours (white, grey, black)."@en;
           skos:definition "Une moisissure est un champignon microscopique. La croissance d’une moisissure peut atteindre des dimensions visibles à l’œil nu sous la forme d’une pellicule duveteuse de diverses couleurs (blanc, gris, noir surtout) ou de filaments croissant depuis un centre (de façon centripète) et formant ainsi un réseau de structures en étoiles, ayant un diamètre de 2 à 10 mm."@en.
:_6bb28298 a skos:Concept;
           skos:inScheme :scheme;
           skos:prefLabel "Plant"@en;
           skos:prefLabel "Plante"@fr;
           skos:altLabel "Higher plant"@en;
           skos:altLabel "vegetation"@en;
           skos:altLabel "Végétation"@fr;
           skos:broader :_94af0e38;
           skos:definition "Vegetal living being, having, when complete, root, stem, and leaves, though consisting sometimes only of a single leafy expansion (e.g. Tree, fern, herb)."@en;
           skos:definition "Etre vivant végétal organisé différencié en racine(s), tige(s) et feuilles. Parfois cependant, la plante peut ne se résumer qu’à une simple expansion foliaire (ex : Fougère, arbre, arbuste, herbe)."@fr.
:_1367e510 a skos:Concept;
           skos:topConceptOf :scheme;
           skos:inScheme :scheme;
           skos:prefLabel "General terms"@en;
           skos:prefLabel "Termes généraux"@fr;
           skos:narrower :_da1c954d;
           skos:narrower :_b6965bcb;
           skos:narrower :_b2cf1a12;
           skos:narrower :_910ffd05;
           skos:narrower :_1eaa61f6;
           skos:narrower :_26e71ab6.
:_da1c954d a skos:Concept;
           skos:inScheme :scheme;
           skos:prefLabel "Decay"@en;
           skos:broader :_1367e510;
           skos:definition "Any chemical or physical modification of the intrin- sic stone properties leading to a loss of value or to the impairment of use"@en.
:_b6965bcb a skos:Concept;
           skos:inScheme :scheme;
           skos:prefLabel "Degradation"@en;
           skos:prefLabel "Dégradation"@fr;
           skos:broader :_1367e510;
           skos:definition "Decline in condition, quality, or functional capacity."@en;
           skos:definition "Toute modification chimique ou physique des pro- priétés intrinsèques de la pierre, conduisant à une perte de valeur, de qualité ou à une entrave à son utilisation."@fr.
:_b2cf1a12 a skos:Concept;
           skos:inScheme :scheme;
           skos:prefLabel "Deterioration"@en;
           skos:altLabel "depreciation"@en;
           skos:broader :_1367e510;
           skos:definition "Process of making or becoming worse or lower in quality, value, character, etc.."@en.
:_910ffd05 a skos:Concept;
           skos:inScheme :scheme;
           skos:prefLabel "Weathering"@en;
           skos:prefLabel "Altération météorique"@fr;
           skos:broader :_1367e510;
           skos:definition "Any chemical or mechanical process by which stones exposed to the weather undergo changes in character and deteriorate."@en;
           skos:definition "Modification des propriétés physicochimiques de la pierre par les agents atmosphériques naturels."@fr.
:_1eaa61f6 a skos:Concept;
           skos:inScheme :scheme;
           skos:prefLabel "Alteration"@en;
           skos:prefLabel "Altération"@fr;
           skos:broader :_1367e510;
           skos:changeNote [
    dct:creator "Nicola Carboni";
    dct:modified "2017-05-26T17:23:54+00:00"
];
           skos:definition "Modification of the material that does not neces- sary imply a worsening of its characteristics from the point of view of conservation. For instance, a reversible coating applied on a stone may be considered as an alteration."@en;
           skos:definition "Modification du matériau n’impliquant pas néces- sairement une dégradation de ses caractéristiques du point de vue de sa conservation. Par exemple, un revêtement réversible appliqué sur une pierre peut être considéré comme une altération."@fr.
:_26e71ab6 a skos:Concept;
           skos:inScheme :scheme;
           skos:prefLabel "Damage"@en;
           skos:broader :_1367e510;
           skos:changeNote [
    dct:creator "Nicola Carboni";
    dct:modified "2017-05-26T18:05:51+00:00"
];
           skos:definition "Human perception of the loss of value due to decay."@en.
